[WIP] Add the isolation proof for another block of code from yield

proof/invariants/Yield.v
@@ -48,248 +48,6 @@ Require Import Invariants GetTableAddr LinkedListConfig PropagatedProperties
                UpdateMappedPageContent InitFstShadow InitSndShadow
                UpdateShadow1StructurePrepare InsertEntryIntoLL. *)
 
-Lemma yield (targetPartDescVAddr : vaddr)
-				    (userTargetInterrupt : userValue)
-				    (userSourceContextSaveIndex : userValue)
-				    (flagsOnYield : interruptMask)
-				    (flagsOnWake : interruptMask)
-				    (sourceInterruptedContext : contextAddr)
-            :
-{{ (* Preconditions *)
-  fun s =>
-  partitionsIsolation s /\
-  kernelDataIsolation s /\
-  verticalSharing s /\
-  consistency s
-}}
-
-checkIntLevelCont targetPartDescVAddr userTargetInterrupt userSourceContextSaveIndex
-                  flagsOnYield flagsOnWake sourceInterruptedContext
-
-{{ (* Postconditions *)
-  fun _ s  =>
-  partitionsIsolation s /\
-  kernelDataIsolation s /\
-  verticalSharing s /\
-  consistency s
-}}.
-
-Proof.
-Admitted.
-
-Definition saveSourceContextCont (targetPartDesc           : page)
-                                 (targetPageDir            : page)
-                                 (sourcePageDir            : page)
-                                 (sourceContextSaveVAddr   : vaddr)
-                                 (nbL                      : level)
-                                 (flagsOnYield             : interruptMask)
-                                 (flagsOnWake              : interruptMask)
-                                 (sourceInterruptedContext : contextAddr)
-                                 (targetContext            : contextAddr)
-                                 (* Needed by the proof *)
-                                 (sourcePartDesc           : page)
-                                 :
-{{ (* Preconditions *)
-  fun s =>
-  partitionsIsolation s /\
-  kernelDataIsolation s /\
-  verticalSharing s /\
-  consistency s /\
-  Some nbL = StateLib.getNbLevel /\
-  List.In sourcePartDesc (StateLib.getPartitions multiplexer s) /\
-  StateLib.nextEntryIsPP sourcePartDesc PDidx sourcePageDir s
-}}
-
-saveSourceContextCont targetPartDesc targetPageDir sourcePageDir
-                      sourceContextSaveVAddr nbL flagsOnYield
-                      flagsOnWake sourceInterruptedContext
-                      targetContext
-{{ (* Postconditions *)
-  fun _ s  =>
-  partitionsIsolation s /\
-  kernelDataIsolation s /\
-  verticalSharing s /\
-  consistency s
-}}.
-Proof.
-unfold saveSourceContextCont.
-
-(* sourceCtxLastMMUPage := getTableAddr sourcePageDir sourceContextSaveVAddr nbL *)
-eapply WP.bindRev.
-eapply WP.weaken.
-eapply (getTableAddr sourcePageDir sourceContextSaveVAddr nbL _ sourcePartDesc PDidx).
-cbn.
-intros s preconditions.
-split.
-apply preconditions.
-destruct preconditions as ( _ & _ & _ & H_cons & H_nbL & H_srcPartDesc & H_srcPageDir ).
-do 3 (split; trivial).
-intuition.
-exists sourcePageDir.
-split; try assumption.
-(* clear H_srcPageDir. *)
-split;[ | intuition ].
-clear H_nbL.
-
-unfold consistency in H_cons.
-unfold partitionDescriptorEntry in H_cons.
-destruct H_cons as (H_partDescEntry & _).
-generalize (H_partDescEntry sourcePartDesc H_srcPartDesc); clear H_partDescEntry; intro H_partDescEntry.
-clear H_srcPartDesc.
-assert (PDidx = PDidx \/ PDidx = sh1idx \/ PDidx = sh2idx \/  PDidx  = sh3idx
-  \/  PDidx  = PPRidx \/  PDidx = PRidx) as H_idxMatch by intuition.
-generalize (H_partDescEntry PDidx H_idxMatch); clear H_partDescEntry; intro H_partDescEntry.
-clear H_idxMatch.
-destruct H_partDescEntry as ( H_validIdx & _ & H_entry ).
-destruct H_entry as (page1 & Hpd & Hnotnull).
-unfold StateLib.nextEntryIsPP in *.
-destruct (StateLib.Index.succ PDidx); try now contradict H_srcPageDir.
-destruct (lookup sourcePartDesc i (memory s) beqPage beqIndex);
-         try now contradict H_srcPageDir.
-destruct v ; try now contradict H_srcPageDir.
-subst; assumption.
-
-cbn.
-intro sourceCtxLastMMUPage.
-(* Postcondition simplification *)
-eapply WP.weaken.
-2: {
-  intros s postconditions.
-  destruct postconditions as (H_initPreconditions & H_addProp).
-  assert ( StateLib.getTableAddrRoot' sourceCtxLastMMUPage PDidx sourcePartDesc sourceContextSaveVAddr s
-           /\ sourceCtxLastMMUPage = defaultPage
-        \/ StateLib.getTableAddrRoot sourceCtxLastMMUPage PDidx sourcePartDesc sourceContextSaveVAddr s
-           /\ sourceCtxLastMMUPage <> defaultPage /\
-            (forall idx : index,
-             StateLib.getIndexOfAddr sourceContextSaveVAddr fstLevel = idx ->
-             StateLib.isPE sourceCtxLastMMUPage idx s)) as H_cleanedPost.
-  {
-    destruct H_addProp as [ ( H_getTableAddr & H_nullSrcCtxLastMMUPage )
-                          | ( H_getTableAddr & H_notNullSrcCtxLastMMUPage & H_entryType) ].
-    + left. split; trivial.
-    + right. do 2 (try split; trivial).
-      intros idx H_getIndexAddr.
-      generalize (H_entryType idx H_getIndexAddr); clear H_entryType; intro H_entryType.
-      destruct H_entryType as [ ( _ & Hfalse ) | [ ( _ & Hfalse ) | ( H_PE & _ ) ] ].
-      - contradict Hfalse.
-        apply InternalLemmas.idxPDidxSh1notEq.
-      - contradict Hfalse.
-        apply DependentTypeLemmas.idxPDidxSh2notEq.
-      - assumption.
-  }
-  clear H_addProp.
-  assert (H_newPost := conj H_initPreconditions H_cleanedPost).
-  pattern s in H_newPost.
-  eapply H_newPost.
-}
-
-(* sourceCtxLastMMUPageIsNull := comparePageToNull sourceCtxLastMMUPage *)
-eapply WP.bindRev.
-eapply Invariants.comparePageToNull.
-intro sourceCtxLastMMUPageIsNull. cbn.
-case_eq sourceCtxLastMMUPageIsNull.
-{ intros.
-  eapply WP.weaken.
-  eapply WP.ret.
-  simpl. intros.
-  intuition.
-}
-intros H_srcCtxLastMMUPageIsNotNull.
-subst.
-
-(* Postcondition simplification *)
-eapply WP.weaken.
-2: {
-  intros s postconditions.
-  destruct postconditions as ( (H_initPreconditions & H_postGetTableAddr ) & H_srcCtxLastMMUPageIsNotNull).
-  apply EqNat.beq_nat_false in H_srcCtxLastMMUPageIsNotNull.
-  assert (StateLib.getTableAddrRoot sourceCtxLastMMUPage PDidx sourcePartDesc sourceContextSaveVAddr s
-       /\ sourceCtxLastMMUPage <> defaultPage
-       /\ (forall idx : index,
-          StateLib.getIndexOfAddr sourceContextSaveVAddr fstLevel = idx ->
-          StateLib.isPE sourceCtxLastMMUPage idx s)) as H_cleanedPost.
-  {
-    destruct H_postGetTableAddr as
-      [ ( H_getTableAddr & H_nullSrcCtxLastMMUPage )
-      | ( H_getTableAddr & H_notNullSrcCtxLastMMUPage & H_entryType) ].
-    + symmetry in H_nullSrcCtxLastMMUPage.
-      contradict H_srcCtxLastMMUPageIsNotNull.
-      f_equal. assumption.
-    + do 2 (try split; trivial).
-  }
-  clear H_postGetTableAddr H_srcCtxLastMMUPageIsNotNull.
-  assert (H_newPost := conj H_initPreconditions H_cleanedPost).
-  try repeat rewrite and_assoc in H_newPost.
-  pattern s in H_newPost.
-  eapply H_newPost.
-}
-
-(* idxSourceCtxInLastMMUPage := MAL.getIndexOfAddr sourceContextSaveVAddr fstLevel *)
-eapply bindRev.
-apply Invariants.getIndexOfAddr.
-intro idxSourceCtxInLastMMUPage.
-cbn.
-
-(* sourceCtxPageIsPresent := MAL.readPresent sourceCtxLastMMUPage idxSourceCtxInLastMMUPage *)
-eapply bindRev.
-eapply weaken.
-apply Invariants.readPresent.
-cbn.
-
-intros s preconditions.
-try repeat rewrite and_assoc in preconditions.
-split.
-apply preconditions.
-destruct preconditions as ( _ & _ & _ & _ & _ & _ & _ & _ & _ & H_isPE & H_getIdxOfAddr ).
-apply H_isPE; assumption.
-
-intro sourceCtxPageIsPresent.
-cbn.
-
-(* if negb sourceCtxPageIsPresent
-   then Hardware.ret IAL.FAIL_CALLER_CONTEXT_SAVE *)
-case_eq (negb sourceCtxPageIsPresent).
-{ intros.
-  eapply WP.weaken.
-  eapply WP.ret.
-  simpl. intros.
-  intuition.
-}
-intros H_srcCtxPageIsPresent.
-apply Bool.negb_false_iff in H_srcCtxPageIsPresent.
-subst.
-
-(* sourceCtxPageIsAccessible := MAL.readAccessible sourceCtxLastMMUPage idxSourceCtxInLastMMUPage *)
-eapply bindRev.
-eapply weaken.
-apply Invariants.readAccessible.
-cbn.
-intros s preconditions.
-try repeat rewrite and_assoc in preconditions.
-split.
-apply preconditions.
-destruct preconditions as ( _ & _ & _ & _ & _ & _ & _ & _ & _ & H_isPE & H_getIdxOfAddr & _ ).
-apply H_isPE; assumption.
-
-intro sourceCtxPageIsAccessible.
-cbn.
-
-(* if negb sourceCtxPageIsAccessible
-   then Hardware.ret IAL.FAIL_CALLER_CONTEXT_SAVE *)
-case_eq (negb sourceCtxPageIsAccessible).
-{ intros.
-  eapply WP.weaken.
-  eapply WP.ret.
-  simpl. intros.
-  intuition.
-}
-
-intro H_sourceCtxPageIsAccessible.
-apply Bool.negb_false_iff in H_sourceCtxPageIsAccessible.
-subst.
-
-Admitted.
-
 Lemma switchContextCont (targetPartDesc : page)
                         (targetPageDir  : page)
                         (flagsOnYield   : interruptMask)
@@ -415,102 +173,989 @@ intros s precondition.
 intuition.
 Qed.
 
-(* 
-set (H_isolation := (fun s : state =>
-            partitionsIsolation s /\ kernelDataIsolation s /\
-            verticalSharing s /\ consistency s
-         )).
+Definition saveSourceContextCont (targetPartDesc           : page)
+                                 (targetPageDir            : page)
+                                 (sourcePageDir            : page)
+                                 (sourceContextSaveVAddr   : vaddr)
+                                 (nbL                      : level)
+                                 (flagsOnYield             : interruptMask)
+                                 (flagsOnWake              : interruptMask)
+                                 (sourceInterruptedContext : contextAddr)
+                                 (targetContext            : contextAddr)
+                                 (* Needed by the proof *)
+                                 (sourcePartDesc           : page)
+                                 :
+{{ (* Preconditions *)
+  fun s =>
+  partitionsIsolation s /\
+  kernelDataIsolation s /\
+  verticalSharing s /\
+  consistency s /\
+  List.In targetPartDesc (StateLib.getPartitions multiplexer s) /\
+  targetPartDesc <> defaultPage /\
+  Some nbL = StateLib.getNbLevel /\
+  List.In sourcePartDesc (StateLib.getPartitions multiplexer s) /\
+  StateLib.nextEntryIsPP sourcePartDesc PDidx sourcePageDir s
+}}
+
+saveSourceContextCont targetPartDesc targetPageDir sourcePageDir
+                      sourceContextSaveVAddr nbL flagsOnYield
+                      flagsOnWake sourceInterruptedContext
+                      targetContext
+{{ (* Postconditions *)
+  fun _ s  =>
+  partitionsIsolation s /\
+  kernelDataIsolation s /\
+  verticalSharing s /\
+  consistency s
+}}.
+Proof.
+unfold saveSourceContextCont.
+
+(* sourceCtxLastMMUPage := getTableAddr sourcePageDir sourceContextSaveVAddr nbL *)
 eapply WP.bindRev.
-instantiate (1:= fun _ s => H_isolation s).
 eapply WP.weaken.
-apply Invariants.updateCurPartition.
+eapply (getTableAddr sourcePageDir sourceContextSaveVAddr nbL _ sourcePartDesc PDidx).
+cbn.
+intros s preconditions.
+split.
+apply preconditions.
+destruct preconditions as ( _ & _ & _ & H_cons & _ & _ & H_nbL & H_srcPartDesc & H_srcPageDir ).
+do 3 (split; trivial).
+intuition.
+exists sourcePageDir.
+split; try assumption.
+split;[ | intuition ].
+clear H_nbL.
+
+unfold consistency in H_cons.
+unfold partitionDescriptorEntry in H_cons.
+destruct H_cons as (H_partDescEntry & _).
+generalize (H_partDescEntry sourcePartDesc H_srcPartDesc); clear H_partDescEntry; intro H_partDescEntry.
+clear H_srcPartDesc.
+assert (PDidx = PDidx \/ PDidx = sh1idx \/ PDidx = sh2idx \/  PDidx  = sh3idx
+  \/  PDidx  = PPRidx \/  PDidx = PRidx) as H_idxMatch by intuition.
+generalize (H_partDescEntry PDidx H_idxMatch); clear H_partDescEntry; intro H_partDescEntry.
+clear H_idxMatch.
+destruct H_partDescEntry as ( H_validIdx & _ & H_entry ).
+destruct H_entry as (page1 & Hpd & Hnotnull).
+unfold StateLib.nextEntryIsPP in *.
+destruct (StateLib.Index.succ PDidx); try now contradict H_srcPageDir.
+destruct (lookup sourcePartDesc i (memory s) beqPage beqIndex);
+         try now contradict H_srcPageDir.
+destruct v ; try now contradict H_srcPageDir.
+subst; assumption.
 
 cbn.
-intro s.
-set (s' := {| currentPartition := targetPartDesc; memory := memory s |}).
-apply updateCurPartitionToPartition.
+intro sourceCtxLastMMUPage.
+(* Postcondition simplification *)
+eapply WP.weaken.
+2: {
+  intros s postconditions.
+  destruct postconditions as (H_initPreconditions & H_addProp).
+  assert ( StateLib.getTableAddrRoot' sourceCtxLastMMUPage PDidx sourcePartDesc sourceContextSaveVAddr s
+           /\ sourceCtxLastMMUPage = defaultPage
+        \/ StateLib.getTableAddrRoot sourceCtxLastMMUPage PDidx sourcePartDesc sourceContextSaveVAddr s
+           /\ sourceCtxLastMMUPage <> defaultPage /\
+            (forall idx : index,
+             StateLib.getIndexOfAddr sourceContextSaveVAddr fstLevel = idx ->
+             StateLib.isPE sourceCtxLastMMUPage idx s)) as H_cleanedPost.
+  {
+    destruct H_addProp as [ ( H_getTableAddr & H_nullSrcCtxLastMMUPage )
+                          | ( H_getTableAddr & H_notNullSrcCtxLastMMUPage & H_entryType) ].
+    + left. split; trivial.
+    + right. do 2 (try split; trivial).
+      intros idx H_getIndexAddr.
+      generalize (H_entryType idx H_getIndexAddr); clear H_entryType; intro H_entryType.
+      destruct H_entryType as [ ( _ & Hfalse ) | [ ( _ & Hfalse ) | ( H_PE & _ ) ] ].
+      - contradict Hfalse.
+        apply InternalLemmas.idxPDidxSh1notEq.
+      - contradict Hfalse.
+        apply DependentTypeLemmas.idxPDidxSh2notEq.
+      - assumption.
+  }
+  clear H_addProp.
+  assert (H_newPost := conj H_initPreconditions H_cleanedPost).
+  pattern s in H_newPost.
+  eapply H_newPost.
+}
 
-(* proof that changing the current partition in the state does not break isolation *)
-intros H_s_isolation.
-unfold H_isolation in *.
-destruct H_s_isolation as [H_part [H_kern [H_vert H_cons]]].
-assert (memory s = memory s') as H_same_mem by trivial.
-split; try split; try split; clear H_isolation.
-- clear H_kern H_vert H_cons.
-  apply partitionsIsolationActivate.
-  trivial.
-- clear H_part H_vert H_cons.
-  apply kernelDataIsolationActivate.
-  trivial.
-- clear H_part H_kern H_cons.
-  apply verticalSharingActivate.
-  trivial.
-- clear H_part H_kern H_vert.
-  apply consistencyActivate.
+(* sourceCtxLastMMUPageIsNull := comparePageToNull sourceCtxLastMMUPage *)
+eapply WP.bindRev.
+eapply Invariants.comparePageToNull.
+intro sourceCtxLastMMUPageIsNull. cbn.
+case_eq sourceCtxLastMMUPageIsNull.
+{ intros.
+  eapply WP.weaken.
+  eapply WP.ret.
+  simpl. intros.
+  intuition.
+}
+intros H_srcCtxLastMMUPageIsNotNull.
+subst.
 
-  unfold partitionsIsolation in *.
-  intros parent child1 child2 H_parent_in_part_list H_child1 H_child2 H_diff_children.
-  assert (forall child, StateLib.getUsedPages child s' = StateLib.getUsedPages child s)
-    as H_same_used_pages by admit.
-  replace (StateLib.getUsedPages child1 s') with (StateLib.getUsedPages child1 s)
-    by (rewrite H_same_used_pages; reflexivity).
-  replace (StateLib.getUsedPages child2 s') with (StateLib.getUsedPages child2 s)
-    by (rewrite H_same_used_pages; reflexivity).
-  clear H_same_used_pages.
-  apply H_part with parent; trivial.
-  + assert (forall multiplexer, StateLib.getPartitions multiplexer s' = StateLib.getPartitions multiplexer s)
-      as H_same_part_tree.
-      intro multiplexer.
-      cbn.
-      replace s with {| currentPartition := (currentPartition s); memory := memory s |} by (destruct s; trivial).
-      cbn.
-      unfold s'.
-  unfold StateLib.getPartitions.
-  destruct (nbPage + 1).
-  reflexivity.
-  cbn.
-  f_equal.
-  unfold StateLib.getChildren.
-  destruct StateLib.getNbLevel; trivial.
-  replace (StateLib.getPd multiplexer (memory {| currentPartition := targetPartDesc; memory := memory s |}))
-     with (StateLib.getPd multiplexer (memory {| currentPartition := currentPartition s; memory := memory s |})) by admit.
-  destruct (StateLib.getPd multiplexer (memory {| currentPartition := currentPartition s; memory := memory s |})); trivial.
-  cbn.
-  unfold StateLib.checkChild.
-  destruct (nbLevel - 1).
-  cbn.
-  reflexivity.
-  unfold StateLib.getIndirection. , StateLib.getMappedPage .
-  cbn.
-  replace (StateLib.getIndirection p va level (nbLevel - 1) {| currentPartition := targetPartDesc; memory := memory s |}) with
-  (StateLib.getIndirection p va level (nbLevel - 1) {| currentPartition := (currentPartition s); memory := memory s |}).
-  unfold StateLib.getIndirection.
-  cbn.
-  simpl.
-  reflexivity.
+(* Postcondition simplification *)
+eapply WP.weaken.
+2: {
+  intros s postconditions.
+  destruct postconditions as ( (H_initPreconditions & H_postGetTableAddr ) & H_srcCtxLastMMUPageIsNotNull).
+  apply EqNat.beq_nat_false in H_srcCtxLastMMUPageIsNotNull.
+  assert (StateLib.getTableAddrRoot sourceCtxLastMMUPage PDidx sourcePartDesc sourceContextSaveVAddr s
+       /\ sourceCtxLastMMUPage <> defaultPage
+       /\ (forall idx : index,
+          StateLib.getIndexOfAddr sourceContextSaveVAddr fstLevel = idx ->
+          StateLib.isPE sourceCtxLastMMUPage idx s)) as H_cleanedPost.
+  {
+    destruct H_postGetTableAddr as
+      [ ( H_getTableAddr & H_nullSrcCtxLastMMUPage )
+      | ( H_getTableAddr & H_notNullSrcCtxLastMMUPage & H_entryType) ].
+    + symmetry in H_nullSrcCtxLastMMUPage.
+      contradict H_srcCtxLastMMUPageIsNotNull.
+      f_equal. assumption.
+    + do 2 (try split; trivial).
+  }
+  clear H_postGetTableAddr H_srcCtxLastMMUPageIsNotNull.
+  assert (H_newPost := conj H_initPreconditions H_cleanedPost).
+  repeat rewrite and_assoc in H_newPost.
+  pattern s in H_newPost.
+  eapply H_newPost.
+}
 
+(* idxSourceCtxInLastMMUPage := MAL.getIndexOfAddr sourceContextSaveVAddr fstLevel *)
+eapply bindRev.
+apply Invariants.getIndexOfAddr.
+intro idxSourceCtxInLastMMUPage.
+cbn.
 
-    replace (StateLib.getPartitions multiplexer s) with (StateLib.getPartitions multiplexer s')
-      by (rewrite H_same_part_tree; reflexivity).
-    trivial.
-  + assert (forall parent, StateLib.getChildren parent s' = StateLib.getChildren parent s)
-      as H_same_children by admit.
-    replace (StateLib.getChildren parent s) with (StateLib.getChildren parent s')
-      by (rewrite H_same_children; reflexivity).
-    trivial.
-  + assert (forall parent, StateLib.getChildren parent s' = StateLib.getChildren parent s)
-      as H_same_children by admit.
-    replace (StateLib.getChildren parent s) with (StateLib.getChildren parent s')
-      by (rewrite H_same_children; reflexivity).
-    trivial.
-(* kernel Isolation *)
-- unfold kernelDataIsolation in *.
-  intros part1 part2.
+(* sourceCtxPageIsPresent := MAL.readPresent sourceCtxLastMMUPage idxSourceCtxInLastMMUPage *)
+eapply bindRev.
+eapply weaken.
+apply Invariants.readPresent.
+cbn.
 
+intros s preconditions.
+try repeat rewrite and_assoc in preconditions.
+split.
+apply preconditions.
+repeat rewrite <- and_assoc in preconditions.
+destruct preconditions as ((_ & H_isPE) & H_getIdxOfAddr).
+apply H_isPE; assumption.
+
+intro sourceCtxPageIsPresent.
+cbn.
+
+(* if negb sourceCtxPageIsPresent
+   then Hardware.ret IAL.FAIL_CALLER_CONTEXT_SAVE *)
+case_eq (negb sourceCtxPageIsPresent).
+{ intros.
+  eapply WP.weaken.
+  eapply WP.ret.
+  simpl. intros.
+  intuition.
+}
+intros H_srcCtxPageIsPresent.
+apply Bool.negb_false_iff in H_srcCtxPageIsPresent.
+subst.
+
+(* sourceCtxPageIsAccessible := MAL.readAccessible sourceCtxLastMMUPage idxSourceCtxInLastMMUPage *)
+eapply bindRev.
+eapply weaken.
+apply Invariants.readAccessible.
+cbn.
+intros s preconditions.
+repeat rewrite and_assoc in preconditions.
+split.
+apply preconditions.
+repeat rewrite <- and_assoc in preconditions.
+destruct preconditions as (((_ & H_isPE) & H_getIdxOfAddr) & _).
+apply H_isPE; assumption.
+
+intro sourceCtxPageIsAccessible.
+cbn.
+
+(* if negb sourceCtxPageIsAccessible
+   then Hardware.ret IAL.FAIL_CALLER_CONTEXT_SAVE *)
+case_eq (negb sourceCtxPageIsAccessible).
+{ intros.
+  eapply WP.weaken.
+  eapply WP.ret.
+  simpl. intros.
+  intuition.
+}
+
+intro H_sourceCtxPageIsAccessible.
+apply Bool.negb_false_iff in H_sourceCtxPageIsAccessible.
+subst.
+
+(* sourceContextEndSaveVAddr := IAL.getNthVAddrFrom sourceContextSaveVAddr IAL.contextSizeMinusOne *)
+eapply bindRev.
+eapply weaken.
+apply Invariants.getNthVAddrFrom.
+cbn.
+intros s preconditions.
+repeat rewrite and_assoc in preconditions.
+apply preconditions.
+cbn.
+intro sourceContextEndSaveVAddr.
+
+(* endAddrOverflow := IAL.firstVAddrGreaterThanSecond sourceContextSaveVAddr sourceContextEndSaveVAddr *)
+eapply bindRev.
+eapply weaken.
+apply Invariants.firstVAddrGreaterThanSecond.
+cbn.
+intros s preconditions.
+apply preconditions.
+cbn.
+intro endAddrOverflow.
+
+(* if endAddrOverflow
+   then Hardware.ret IAL.FAIL_CALLER_CONTEXT_SAVE *)
+case_eq endAddrOverflow.
+{ intros.
+  eapply WP.weaken.
+  eapply WP.ret.
+  simpl. intros.
+  intuition.
+}
+intro H_noVAddrOverflow.
+subst.
+
+(* sourceCtxEndLastMMUPage := Internal.getTableAddr sourcePageDir sourceContextEndSaveVAddr nbL *)
+eapply bindRev.
+eapply weaken.
+eapply (getTableAddr sourcePageDir sourceContextEndSaveVAddr nbL _ sourcePartDesc PDidx).
+cbn.
+intros s preconditions.
+split.
+apply preconditions.
+destruct preconditions as ( _ & _ & _ & H_cons & _ & _ & H_nbL & H_srcPartDesc & H_srcPageDir & _ ).
+do 3 (split; trivial).
+intuition.
+exists sourcePageDir.
+split; try assumption.
+split;[ | intuition ].
+clear H_nbL.
+
+unfold consistency in H_cons.
+unfold partitionDescriptorEntry in H_cons.
+destruct H_cons as (H_partDescEntry & _).
+generalize (H_partDescEntry sourcePartDesc H_srcPartDesc); clear H_partDescEntry; intro H_partDescEntry.
+clear H_srcPartDesc.
+assert (PDidx = PDidx \/ PDidx = sh1idx \/ PDidx = sh2idx \/  PDidx  = sh3idx
+  \/  PDidx  = PPRidx \/  PDidx = PRidx) as H_idxMatch by intuition.
+generalize (H_partDescEntry PDidx H_idxMatch); clear H_partDescEntry; intro H_partDescEntry.
+clear H_idxMatch.
+destruct H_partDescEntry as ( H_validIdx & _ & H_entry ).
+destruct H_entry as (page1 & Hpd & Hnotnull).
+unfold StateLib.nextEntryIsPP in *.
+destruct (StateLib.Index.succ PDidx); try now contradict H_srcPageDir.
+destruct (lookup sourcePartDesc i (memory s) beqPage beqIndex);
+         try now contradict H_srcPageDir.
+destruct v ; try now contradict H_srcPageDir.
+subst; assumption.
+
+cbn.
+intro sourceCtxEndLastMMUPage.
+(* Postcondition simplification *)
+eapply WP.weaken.
+2: {
+  intros s postconditions.
+  destruct postconditions as (H_initPreconditions & H_addProp).
+  assert ( StateLib.getTableAddrRoot' sourceCtxEndLastMMUPage PDidx sourcePartDesc sourceContextEndSaveVAddr s
+           /\ sourceCtxEndLastMMUPage = defaultPage
+        \/ StateLib.getTableAddrRoot sourceCtxEndLastMMUPage PDidx sourcePartDesc sourceContextEndSaveVAddr s
+           /\ sourceCtxEndLastMMUPage <> defaultPage /\
+            (forall idx : index,
+             StateLib.getIndexOfAddr sourceContextEndSaveVAddr fstLevel = idx ->
+             StateLib.isPE sourceCtxEndLastMMUPage idx s)) as H_cleanedPost.
+  {
+    destruct H_addProp as [ ( H_getTableAddr & H_nullSrcCtxLastMMUPage )
+                          | ( H_getTableAddr & H_notNullSrcCtxLastMMUPage & H_entryType) ].
+    + left. split; trivial.
+    + right. do 2 (try split; trivial).
+      intros idx H_getIndexAddr.
+      generalize (H_entryType idx H_getIndexAddr); clear H_entryType; intro H_entryType.
+      destruct H_entryType as [ ( _ & Hfalse ) | [ ( _ & Hfalse ) | ( H_PE & _ ) ] ].
+      - contradict Hfalse.
+        apply InternalLemmas.idxPDidxSh1notEq.
+      - contradict Hfalse.
+        apply DependentTypeLemmas.idxPDidxSh2notEq.
+      - assumption.
+  }
+  clear H_addProp.
+  assert (H_newPost := conj H_initPreconditions H_cleanedPost).
+  pattern s in H_newPost.
+  eapply H_newPost.
+}
+
+(* sourceCtxEndLastMMUPageIsNull := comparePageToNull sourceCtxEndLastMMUPage *)
+eapply WP.bindRev.
+eapply Invariants.comparePageToNull.
+intro sourceCtxEndLastMMUPageIsNull. cbn.
+case_eq sourceCtxEndLastMMUPageIsNull.
+{ intros.
+  eapply WP.weaken.
+  eapply WP.ret.
+  simpl. intros.
+  intuition.
+}
+intros H_srcCtxEndLastMMUPageIsNotNull.
+subst.
+
+(* Postcondition simplification *)
+eapply WP.weaken.
+2: {
+  intros s postconditions.
+  destruct postconditions as ( (H_initPreconditions & H_postGetTableAddr ) & H_srcCtxEndLastMMUPageIsNotNull).
+  apply EqNat.beq_nat_false in H_srcCtxEndLastMMUPageIsNotNull.
+  assert (StateLib.getTableAddrRoot sourceCtxEndLastMMUPage PDidx sourcePartDesc sourceContextEndSaveVAddr s
+       /\ sourceCtxEndLastMMUPage <> defaultPage
+       /\ (forall idx : index,
+          StateLib.getIndexOfAddr sourceContextEndSaveVAddr fstLevel = idx ->
+          StateLib.isPE sourceCtxEndLastMMUPage idx s)) as H_cleanedPost.
+  {
+    destruct H_postGetTableAddr as
+      [ ( H_getTableAddr & H_nullSrcCtxEndLastMMUPage )
+      | ( H_getTableAddr & H_notNullSrcCtxEndLastMMUPage & H_entryType) ].
+    + symmetry in H_nullSrcCtxEndLastMMUPage.
+      contradict H_srcCtxEndLastMMUPageIsNotNull.
+      f_equal. assumption.
+    + do 2 (try split; trivial).
+  }
+  clear H_postGetTableAddr H_srcCtxEndLastMMUPageIsNotNull.
+  assert (H_newPost := conj H_initPreconditions H_cleanedPost).
+  repeat rewrite and_assoc in H_newPost.
+  pattern s in H_newPost.
+  eapply H_newPost.
+}
+
+(* idxSourceCtxEndInLastMMUPage := MAL.getIndexOfAddr sourceContextEndSaveVAddr fstLevel *)
+eapply bindRev.
+apply Invariants.getIndexOfAddr.
+intro idxSourceCtxEndInLastMMUPage.
+cbn.
+
+(* sourceCtxEndPageIsPresent := MAL.readPresent sourceCtxEndLastMMUPage idxSourceCtxEndInLastMMUPage *)
+eapply bindRev.
+eapply weaken.
+apply Invariants.readPresent.
+cbn.
+
+intros s preconditions.
+try repeat rewrite and_assoc in preconditions.
+split.
+apply preconditions.
+repeat rewrite <- and_assoc in preconditions.
+destruct preconditions as ((_ & H_isPE) & H_getIdxOfAddr).
+apply H_isPE; assumption.
+
+intro sourceCtxEndPageIsPresent.
+cbn.
+
+(* if negb sourceCtxEndPageIsPresent
+   then Hardware.ret IAL.FAIL_CALLER_CONTEXT_SAVE *)
+case_eq (negb sourceCtxEndPageIsPresent).
+{ intros.
+  eapply WP.weaken.
+  eapply WP.ret.
+  simpl. intros.
+  intuition.
+}
+intros H_srcCtxEndPageIsPresent.
+apply Bool.negb_false_iff in H_srcCtxEndPageIsPresent.
+subst.
+
+(* sourceCtxEndPageIsAccessible := MAL.readAccessible sourceCtxEndLastMMUPage idxSourceCtxEndInLastMMUPage *)
+eapply bindRev.
+eapply weaken.
+apply Invariants.readAccessible.
+cbn.
+intros s preconditions.
+repeat rewrite and_assoc in preconditions.
+split.
+apply preconditions.
+repeat rewrite <- and_assoc in preconditions.
+destruct preconditions as (((_ & H_isPE) & H_getIdxOfAddr) & _ ).
+apply H_isPE; assumption.
+
+intro sourceCtxEndPageIsAccessible.
+cbn.
+
+(* if negb sourceCtxEndPageIsAccessible
+   then Hardware.ret IAL.FAIL_CALLER_CONTEXT_SAVE *)
+case_eq (negb sourceCtxEndPageIsAccessible).
+{ intros.
+  eapply WP.weaken.
+  eapply WP.ret.
+  simpl. intros.
+  intuition.
+}
+
+intro H_sourceCtxEndPageIsAccessible.
+apply Bool.negb_false_iff in H_sourceCtxEndPageIsAccessible.
+subst.
+
+(* IAL.writeContext sourceInterruptedContext sourceContextSaveVAddr flagsOnWake *)
+eapply bindRev.
+eapply weaken.
+apply Invariants.writeContext.
+cbn.
+intros s preconditions.
+repeat rewrite and_assoc in preconditions.
+destruct preconditions as (H_part & H_kern & H_vert & H_cons & H_targetPartDescInPartList
+                         & H_targetPartNotDef & _).
+assert (preconditions := conj H_part
+                        (conj H_kern
+                        (conj H_vert
+                        (conj H_cons
+                        (conj H_targetPartDescInPartList
+                              H_targetPartNotDef
+                        ))))
+       ).
+pattern s in preconditions.
+apply preconditions.
+cbn.
+intro u; clear u.
+
+eapply WP.weaken.
+apply switchContextCont.
+cbn.
+trivial.
+Qed.
+
+Lemma getTargetContextCont (targetPartDesc : page)
+			                     (targetPageDir  : page)
+			                     (targetVidt     : page)
+			                     (sourcePageDir  : page)
+                           (sourceContextSaveVaddr : vaddr)
+			                     (targetInterrupt : index)
+			                     (nbL : level)
+			                     (flagsOnYield   : interruptMask)
+			                     (flagsOnWake    : interruptMask)
+			                     (sourceInterruptedContext : contextAddr)
+                           (* Needed by the proof *)
+                           (sourcePartDesc           : page)
+                           :
+{{ (* Preconditions *)
+  fun s =>
+  partitionsIsolation s /\
+  kernelDataIsolation s /\
+  verticalSharing s /\
+  consistency s /\
+  List.In targetPartDesc (StateLib.getPartitions multiplexer s) /\
+  StateLib.nextEntryIsPP targetPartDesc PDidx targetPageDir s /\
+  targetPartDesc <> defaultPage /\
+  Some nbL = StateLib.getNbLevel /\
+  List.In sourcePartDesc (StateLib.getPartitions multiplexer s) /\
+  StateLib.nextEntryIsPP sourcePartDesc PDidx sourcePageDir s
+}}
+
+getTargetContextCont targetPartDesc targetPageDir targetVidt sourcePageDir
+                     sourceContextSaveVaddr targetInterrupt nbL flagsOnYield
+			               flagsOnWake sourceInterruptedContext
+{{ (* Postconditions *)
+  fun _ s  =>
+  partitionsIsolation s /\
+  kernelDataIsolation s /\
+  verticalSharing s /\
+  consistency s
+}}.
+Proof.
+unfold getTargetContextCont.
+
+(* targetContextVAddr := MAL.readVirtualUser targetVidt targetInterrupt *)
+eapply WP.bindRev.
+eapply WP.weaken.
+apply Invariants.readVirtualUser.
+cbn.
+intros s preconditions.
+apply preconditions.
+cbn.
+intro targetContextVAddr.
+
+(* targetContextLastMMUPage := Internal.getTableAddr targetPageDir targetContextVAddr nbL *)
+eapply WP.bindRev.
+eapply WP.weaken.
+eapply (getTableAddr targetPageDir targetContextVAddr nbL _ targetPartDesc PDidx).
+cbn.
+intros s preconditions.
+repeat rewrite and_assoc in preconditions.
+split.
+apply preconditions.
+destruct preconditions as ( _ & _ & _ & H_cons & H_tgtPartDesc & H_tgtPageDir & _ & H_nbL & _ ).
+do 3 (split; trivial).
+intuition.
+exists targetPageDir.
+split; try assumption.
+split;[ | intuition ].
+clear H_nbL.
+
+unfold consistency in H_cons.
+unfold partitionDescriptorEntry in H_cons.
+destruct H_cons as (H_partDescEntry & _).
+generalize (H_partDescEntry targetPartDesc H_tgtPartDesc); clear H_partDescEntry; intro H_partDescEntry.
+clear H_tgtPartDesc.
+assert (PDidx = PDidx \/ PDidx = sh1idx \/ PDidx = sh2idx \/  PDidx  = sh3idx
+  \/  PDidx  = PPRidx \/  PDidx = PRidx) as H_idxMatch by intuition.
+generalize (H_partDescEntry PDidx H_idxMatch); clear H_partDescEntry; intro H_partDescEntry.
+clear H_idxMatch.
+destruct H_partDescEntry as ( H_validIdx & _ & H_entry ).
+destruct H_entry as (page1 & Hpd & Hnotnull).
+unfold StateLib.nextEntryIsPP in *.
+destruct (StateLib.Index.succ PDidx); try now contradict H_tgtPageDir.
+destruct (lookup targetPartDesc i (memory s) beqPage beqIndex);
+         try now contradict H_tgtPageDir.
+destruct v ; try now contradict H_tgtPageDir.
+subst; assumption.
+
+cbn.
+intro targetContextLastMMUPage.
+(* Postcondition simplification *)
+eapply WP.weaken.
+2: {
+  intros s postconditions.
+  destruct postconditions as (H_initPreconditions & H_addProp).
+  assert ( StateLib.getTableAddrRoot' targetContextLastMMUPage PDidx targetPartDesc targetContextVAddr s
+           /\ targetContextLastMMUPage = defaultPage
+        \/ StateLib.getTableAddrRoot targetContextLastMMUPage PDidx targetPartDesc targetContextVAddr s
+           /\ targetContextLastMMUPage <> defaultPage /\
+            (forall idx : index,
+             StateLib.getIndexOfAddr targetContextVAddr fstLevel = idx ->
+             StateLib.isPE targetContextLastMMUPage idx s)) as H_cleanedPost.
+  {
+    destruct H_addProp as [ ( H_getTableAddr & H_nullTgtCtxLastMMUPage )
+                          | ( H_getTableAddr & H_notNullTgtCtxLastMMUPage & H_entryType) ].
+    + left. split; trivial.
+    + right. do 2 (try split; trivial).
+      intros idx H_getIndexAddr.
+      generalize (H_entryType idx H_getIndexAddr); clear H_entryType; intro H_entryType.
+      destruct H_entryType as [ ( _ & Hfalse ) | [ ( _ & Hfalse ) | ( H_PE & _ ) ] ].
+      - contradict Hfalse.
+        apply InternalLemmas.idxPDidxSh1notEq.
+      - contradict Hfalse.
+        apply DependentTypeLemmas.idxPDidxSh2notEq.
+      - assumption.
+  }
+  clear H_addProp.
+  assert (H_newPost := conj H_initPreconditions H_cleanedPost).
+  pattern s in H_newPost.
+  eapply H_newPost.
+}
+
+(* targetContextLastMMUPageisNull := Internal.comparePageToNull targetContextLastMMUPage *)
+eapply WP.bindRev.
+eapply Invariants.comparePageToNull.
+intro targetContextLastMMUPageIsNull. cbn.
+case_eq targetContextLastMMUPageIsNull.
+{ intros.
+  eapply WP.weaken.
+  eapply WP.ret.
+  simpl. intros.
+  intuition.
+}
+intros H_targetContextLastMMUPageIsNull.
+subst.
+
+(* Postcondition simplification *)
+eapply WP.weaken.
+2: {
+  intros s postconditions.
+  destruct postconditions as ( (H_initPreconditions & H_postGetTableAddr ) & H_targetContextLastMMUPageIsNotNull).
+  apply EqNat.beq_nat_false in H_targetContextLastMMUPageIsNotNull.
+  assert (StateLib.getTableAddrRoot targetContextLastMMUPage PDidx targetPartDesc targetContextVAddr s
+       /\ targetContextLastMMUPage <> defaultPage
+       /\ (forall idx : index,
+          StateLib.getIndexOfAddr targetContextVAddr fstLevel = idx ->
+          StateLib.isPE targetContextLastMMUPage idx s)) as H_cleanedPost.
+  {
+    destruct H_postGetTableAddr as
+      [ ( H_getTableAddr & H_nullTgtCtxLastMMUPage )
+      | ( H_getTableAddr & H_notNullTgtCtxLastMMUPage & H_entryType) ].
+    + symmetry in H_nullTgtCtxLastMMUPage.
+      contradict H_targetContextLastMMUPageIsNotNull.
+      f_equal. assumption.
+    + do 2 (try split; trivial).
+  }
+  clear H_postGetTableAddr H_targetContextLastMMUPageIsNotNull.
+  assert (H_newPost := conj H_initPreconditions H_cleanedPost).
+  repeat rewrite and_assoc in H_newPost.
+  pattern s in H_newPost.
+  eapply H_newPost.
+}
+
+(* idxTargetContextPageInLastMMUPage := MAL.getIndexOfAddr targetContextVAddr fstLevel *)
+eapply WP.bindRev.
+eapply Invariants.getIndexOfAddr.
+cbn.
+intro idxTargetContextPageInLastMMUPage.
+
+(* targetContextPageIsPresent := MAL.readPresent targetContextLastMMUPage idxTargetContextPageInLastMMUPage *)
+eapply bindRev.
+eapply weaken.
+apply Invariants.readPresent.
+cbn.
+
+intros s preconditions.
+try repeat rewrite and_assoc in preconditions.
+split.
+apply preconditions.
+repeat rewrite <- and_assoc in preconditions.
+destruct preconditions as ((_ & H_isPE) & H_getIdxOfAddr).
+apply H_isPE; assumption.
+
+intro targetContextPageIsPresent.
+cbn.
+
+(* if negb targetContextPageIsPresent
+   then Hardware.ret IAL.FAIL_UNAVAILABLE_TARGET_CTX *)
+case_eq (negb targetContextPageIsPresent).
+{ intros.
+  eapply WP.weaken.
+  eapply WP.ret.
+  simpl. intros.
+  intuition.
+}
+intros H_targetContextPageIsPresent.
+apply Bool.negb_false_iff in H_targetContextPageIsPresent.
+subst.
+
+(* targetContextPageIsAccessible := MAL.readAccessible targetContextLastMMUPage idxTargetContextPageInLastMMUPage *)
+eapply bindRev.
+eapply weaken.
+apply Invariants.readAccessible.
+cbn.
+intros s preconditions.
+repeat rewrite and_assoc in preconditions.
+split.
+apply preconditions.
+repeat rewrite <- and_assoc in preconditions.
+destruct preconditions as (((_ & H_isPE) & H_getIdxOfAddr) & _ ).
+apply H_isPE; assumption.
+
+intro targetContextPageIsAccessible.
+cbn.
+
+(* if negb targetContextPageIsAccessible
+   then Hardware.ret IAL.FAIL_UNAVAILABLE_TARGET_CTX *)
+case_eq (negb targetContextPageIsAccessible).
+{ intros.
+  eapply WP.weaken.
+  eapply WP.ret.
+  simpl. intros.
+  intuition.
+}
+
+intro H_targetContextPageIsAccessible.
+apply Bool.negb_false_iff in H_targetContextPageIsAccessible.
+subst.
+
+(* targetContextEndVAddr := IAL.getNthVAddrFrom targetContextVAddr IAL.contextSizeMinusOne *)
+eapply bindRev.
+eapply weaken.
+apply Invariants.getNthVAddrFrom.
+cbn.
+intros s preconditions.
+repeat rewrite and_assoc in preconditions.
+apply preconditions.
+cbn.
+intro targetContextEndVAddr.
+
+(* targetContextEndVAddrOverflow := IAL.firstVAddrGreaterThanSecond targetContextVAddr targetContextEndVAddr *)
+eapply bindRev.
+eapply weaken.
+apply Invariants.firstVAddrGreaterThanSecond.
+cbn.
+intros s preconditions.
+apply preconditions.
+cbn.
+intro endAddrOverflow.
+
+(* if endAddrOverflow
+   then Hardware.ret IAL.FAIL_UNAVAILABLE_TARGET_CTX *)
+case_eq endAddrOverflow.
+{ intros.
+  eapply WP.weaken.
+  eapply WP.ret.
+  simpl. intros.
+  intuition.
+}
+intro H_noVAddrOverflow.
+subst.
+
+(* targetContextEndLastMMUPage := Internal.getTableAddr targetPageDir targetContextEndVAddr nbL *)
+eapply bindRev.
+eapply weaken.
+eapply (getTableAddr targetPageDir targetContextEndVAddr nbL _ targetPartDesc PDidx).
+cbn.
+intros s preconditions.
+split.
+apply preconditions.
+destruct preconditions as ( _ & _ & _ & H_cons & H_tgtPartDesc & H_tgtPageDir & _ & H_nbL & _ ).
+do 3 (split; trivial).
+intuition.
+exists targetPageDir.
+split; try assumption.
+split;[ | intuition ].
+clear H_nbL.
+
+unfold consistency in H_cons.
+unfold partitionDescriptorEntry in H_cons.
+destruct H_cons as (H_partDescEntry & _).
+generalize (H_partDescEntry targetPartDesc H_tgtPartDesc); clear H_partDescEntry; intro H_partDescEntry.
+clear H_tgtPartDesc.
+assert (PDidx = PDidx \/ PDidx = sh1idx \/ PDidx = sh2idx \/  PDidx  = sh3idx
+  \/  PDidx  = PPRidx \/  PDidx = PRidx) as H_idxMatch by intuition.
+generalize (H_partDescEntry PDidx H_idxMatch); clear H_partDescEntry; intro H_partDescEntry.
+clear H_idxMatch.
+destruct H_partDescEntry as ( H_validIdx & _ & H_entry ).
+destruct H_entry as (page1 & Hpd & Hnotnull).
+unfold StateLib.nextEntryIsPP in *.
+destruct (StateLib.Index.succ PDidx); try now contradict H_tgtPageDir.
+destruct (lookup targetPartDesc i (memory s) beqPage beqIndex);
+         try now contradict H_tgtPageDir.
+destruct v ; try now contradict H_tgtPageDir.
+subst; assumption.
+
+cbn.
+intro targetContextEndLastMMUPage.
+(* Postcondition simplification *)
+eapply WP.weaken.
+2: {
+  intros s postconditions.
+  destruct postconditions as (H_initPreconditions & H_addProp).
+  assert ( StateLib.getTableAddrRoot' targetContextEndLastMMUPage PDidx targetPartDesc targetContextEndVAddr s
+           /\ targetContextEndLastMMUPage = defaultPage
+        \/ StateLib.getTableAddrRoot targetContextEndLastMMUPage PDidx targetPartDesc targetContextEndVAddr s
+           /\ targetContextEndLastMMUPage <> defaultPage /\
+            (forall idx : index,
+             StateLib.getIndexOfAddr targetContextEndVAddr fstLevel = idx ->
+             StateLib.isPE targetContextEndLastMMUPage idx s)) as H_cleanedPost.
+  {
+    destruct H_addProp as [ ( H_getTableAddr & H_nullTgtCtxEndLastMMUPage )
+                          | ( H_getTableAddr & H_notNullTgtCtxEndLastMMUPage & H_entryType) ].
+    + left. split; trivial.
+    + right. do 2 (try split; trivial).
+      intros idx H_getIndexAddr.
+      generalize (H_entryType idx H_getIndexAddr); clear H_entryType; intro H_entryType.
+      destruct H_entryType as [ ( _ & Hfalse ) | [ ( _ & Hfalse ) | ( H_PE & _ ) ] ].
+      - contradict Hfalse.
+        apply InternalLemmas.idxPDidxSh1notEq.
+      - contradict Hfalse.
+        apply DependentTypeLemmas.idxPDidxSh2notEq.
+      - assumption.
+  }
+  clear H_addProp.
+  assert (H_newPost := conj H_initPreconditions H_cleanedPost).
+  pattern s in H_newPost.
+  eapply H_newPost.
+}
+
+(* targetContextEndLastMMUPageisNull := Internal.comparePageToNull targetContextEndLastMMUPage *)
+eapply WP.bindRev.
+eapply Invariants.comparePageToNull.
+intro targetContextEndLastMMUPageisNull. cbn.
+case_eq targetContextEndLastMMUPageisNull.
+{ intros.
+  eapply WP.weaken.
+  eapply WP.ret.
+  simpl. intros.
+  intuition.
+}
+intros H_tgtCtxEndLastMMUPageIsNotNull.
+subst.
+
+(* Postcondition simplification *)
+eapply WP.weaken.
+2: {
+  intros s postconditions.
+  destruct postconditions as ( (H_initPreconditions & H_postGetTableAddr ) & H_tgtCtxEndLastMMUPageIsNotNull).
+  apply EqNat.beq_nat_false in H_tgtCtxEndLastMMUPageIsNotNull.
+  assert (StateLib.getTableAddrRoot targetContextEndLastMMUPage PDidx targetPartDesc targetContextEndVAddr s
+       /\ targetContextEndLastMMUPage <> defaultPage
+       /\ (forall idx : index,
+          StateLib.getIndexOfAddr targetContextEndVAddr fstLevel = idx ->
+          StateLib.isPE targetContextEndLastMMUPage idx s)) as H_cleanedPost.
+  {
+    destruct H_postGetTableAddr as
+      [ ( H_getTableAddr & H_nullTgtCtxEndLastMMUPage )
+      | ( H_getTableAddr & H_notNullTgtCtxEndLastMMUPage & H_entryType) ].
+    + symmetry in H_nullTgtCtxEndLastMMUPage.
+      contradict H_tgtCtxEndLastMMUPageIsNotNull.
+      f_equal. assumption.
+    + do 2 (try split; trivial).
+  }
+  clear H_postGetTableAddr H_tgtCtxEndLastMMUPageIsNotNull.
+  assert (H_newPost := conj H_initPreconditions H_cleanedPost).
+  repeat rewrite and_assoc in H_newPost.
+  pattern s in H_newPost.
+  eapply H_newPost.
+}
+
+(* idxTargetContextEndPageInLastMMUPage := MAL.getIndexOfAddr targetContextEndVAddr fstLevel *)
+eapply bindRev.
+apply Invariants.getIndexOfAddr.
+intro idxTargetContextEndPageInLastMMUPage.
+cbn.
+
+(* targetContextEndPageIsPresent := MAL.readPresent targetContextEndLastMMUPage idxSourceCtxEndInLastMMUPage *)
+eapply bindRev.
+eapply weaken.
+apply Invariants.readPresent.
+cbn.
+
+intros s preconditions.
+try repeat rewrite and_assoc in preconditions.
+split.
+apply preconditions.
+repeat rewrite <- and_assoc in preconditions.
+destruct preconditions as ((_ & H_isPE) & H_getIdxOfAddr).
+apply H_isPE; assumption.
+
+intro targetContextEndPageIsPresent.
+cbn.
+
+(* if negb targetContextEndPageIsPresent
+   then Hardware.ret IAL.FAIL_UNAVAILABLE_TARGET_CTX *)
+case_eq (negb targetContextEndPageIsPresent).
+{ intros.
+  eapply WP.weaken.
+  eapply WP.ret.
+  simpl. intros.
+  intuition.
+}
+intros H_targetContextEndPageIsPresent.
+apply Bool.negb_false_iff in H_targetContextEndPageIsPresent.
+subst.
+
+(* targetContextEndPageIsAccessible := MAL.readAccessible targetContextEndLastMMUPage idxTargetContextEndPageInLastMMUPage *)
+eapply bindRev.
+eapply weaken.
+apply Invariants.readAccessible.
+cbn.
+intros s preconditions.
+repeat rewrite and_assoc in preconditions.
+split.
+apply preconditions.
+repeat rewrite <- and_assoc in preconditions.
+destruct preconditions as (((_ & H_isPE) & H_getIdxOfAddr) & _ ).
+apply H_isPE; assumption.
+
+intro targetContextEndPageIsAccessible.
+cbn.
+
+(* if negb targetContextEndPageIsAccessible
+   then Hardware.ret IAL.FAIL_UNAVAILABLE_TARGET_CTX *)
+case_eq (negb targetContextEndPageIsAccessible).
+{ intros.
+  eapply WP.weaken.
+  eapply WP.ret.
+  simpl. intros.
+  intuition.
+}
+
+intro H_targetContextEndPageIsAccessible.
+apply Bool.negb_false_iff in H_targetContextEndPageIsAccessible.
+subst.
+
+(* targetContext := IAL.vaddrToContextAddr targetContextVAddr *)
+eapply WP.bindRev.
+eapply WP.weaken.
+apply Invariants.vaddrToContextAddr.
+cbn.
+intros s preconditions.
+repeat rewrite and_assoc in preconditions.
+apply preconditions.
+cbn.
+
+intro targetContext.
+
+(* sourceContextSaveVaddrIsNull := Internal.compareVAddrToNull sourceContextSaveVaddr *)
+eapply WP.bindRev.
+eapply WP.weaken.
+apply Invariants.compareVAddrToNull.
+cbn.
+intros s preconditions.
+apply preconditions.
+intro sourceContextSaveVaddrIsNull. cbn.
+case_eq sourceContextSaveVaddrIsNull.
+{ intros.
+  eapply WP.weaken.
+  apply (switchContextCont targetPartDesc targetPageDir flagsOnYield targetContext).
+  intros s preconditions.
+  cbn.
+  intuition.
+}
+{
+  intros.
+  eapply WP.weaken.
+  apply (saveSourceContextCont targetPartDesc targetPageDir sourcePageDir sourceContextSaveVaddr nbL
+         flagsOnYield flagsOnWake sourceInterruptedContext targetContext sourcePartDesc).
+  intros s preconditions.
+  cbn.
+  intuition.
+}
+Qed.
+
+Lemma getTargetVidtCont (targetPartDesc : page)
+	                      (sourcePageDir : page)
+		                    (vidtVAddr : vaddr)
+		                    (sourceContextSaveVAddr : vaddr)
+		                    (targetInterrupt : index)
+		                    (nbL : level)
+		                    (idxVidtInLastMMUPage : index)
+		                    (flagsOnYield : interruptMask)
+		                    (flagsOnWake : interruptMask)
+		                    (sourceInterruptedContext : contextAddr)
+                        (* Needed by the proof *)
+                        (sourcePartDesc           : page)
+                        :
+{{ (* Preconditions *)
+  fun s =>
+  partitionsIsolation s /\
+  kernelDataIsolation s /\
+  verticalSharing s /\
+  consistency s
+}}
+
+getTargetVidtCont targetPartDesc sourcePageDir vidtVAddr sourceContextSaveVAddr targetInterrupt
+                  nbL idxVidtInLastMMUPage flagsOnYield flagsOnWake sourceInterruptedContext
+
+{{ (* Postconditions *)
+  fun _ s  =>
+  partitionsIsolation s /\
+  kernelDataIsolation s /\
+  verticalSharing s /\
+  consistency s
+}}.
+Proof.
 Admitted.
- *)
 
+Lemma yield (targetPartDescVAddr : vaddr)
+				    (userTargetInterrupt : userValue)
+				    (userSourceContextSaveIndex : userValue)
+				    (flagsOnYield : interruptMask)
+				    (flagsOnWake : interruptMask)
+				    (sourceInterruptedContext : contextAddr)
+            :
+{{ (* Preconditions *)
+  fun s =>
+  partitionsIsolation s /\
+  kernelDataIsolation s /\
+  verticalSharing s /\
+  consistency s
+}}
 
+checkIntLevelCont targetPartDescVAddr userTargetInterrupt userSourceContextSaveIndex
+                  flagsOnYield flagsOnWake sourceInterruptedContext
 
+{{ (* Postconditions *)
+  fun _ s  =>
+  partitionsIsolation s /\
+  kernelDataIsolation s /\
+  verticalSharing s /\
+  consistency s
+}}.
 
+Proof.
+Admitted.
 
